beginning to get GC structure right

disk-betree/BlockCache.dfy
@@ -1,14 +1,14 @@
 include "../lib/Maps.dfy"
 include "../lib/sequences.dfy"
   
-abstract module BlockCache {
+abstract module BlockInterface {
   import opened Sequences
   import opened Maps
     
-  type Reference(!new,==)
+  type Reference(!new,==) // LBA
 
   type View<T> = imap<Reference, T>
-  type ReferenceTree = imap<Reference, set<Reference>>
+  type ReferenceTree = imap<Reference, iset<Reference>>
 
   function Root(k: Constants) : Reference
 
@@ -21,6 +21,7 @@ abstract module BlockCache {
   {
     && |lookup| > 0
     && lookup[0] == Root(k)
+    && (forall i :: 0 <= i < |lookup| ==> lookup[i] in s.reftree)
     && (forall i :: 0 <= i < |lookup|-1 ==> lookup[i+1] in s.reftree[lookup[i]])
   }
 
@@ -29,44 +30,89 @@ abstract module BlockCache {
     exists lookup :: LookupIsValid(k, s, lookup) && Last(lookup) == ref
   }
 
-  function LiveReferences(k: Constants, s: Variables) : set<Reference> {
-    set ref | ReachableReference(k, s, ref)
+  function LiveReferences(k: Constants, s: Variables) : iset<Reference> {
+    iset ref | ReachableReference(k, s, ref)
   }
 
+  predicate LiveDataAvailable(k: Constants, s: Variables) {
+    LiveReferences(k, s) <= s.view.Keys
+  }
   
-  function ViewOf<T>(k: Constants, s: Variables) : View
-  
-  // function Read<T>(k: Constants, s: Variables, ref: Reference) : T
-  //   requires ref in ViewOf(k, s)
-  //   ensures Read(k, s, ref) == ViewOf(k, s)[ref];
+  function Read<T>(k: Constants, s: Variables, ref: Reference) : T
+    requires LiveDataAvailable(k, s)
+    requires ReachableReference(k, s, ref)
+  {
+    s.view[ref]
+  }
     
   datatype CacheOp<T> =
     | AllocOp(block: T, successors: iset<Reference>, ref: Reference)
     | WriteOp(ref: Reference, block: T, successors: iset<Reference>)
+
+  function ApplyToReferenceTree(reftree: ReferenceTree, op: CacheOp) : ReferenceTree {
+    reftree[op.ref := op.successors]
+  }
     
   function ApplyToView(view: View, op: CacheOp) : View {
     view[op.ref := op.block]
   }
     
-  predicate Apply(k: Constants, s: Variables, s': Variables, op: CacheOp)
-    ensures Apply(k, s, s', op) ==> ViewOf(k, s') == ApplyToView(ViewOf(k, s), op)
-    ensures op.AllocOp? && Apply(k, s, s', op) ==> op.ref !in LiveReferences(k, s)
-    ensures op.WriteOp? && Apply(k, s, s', op) ==> op.ref in LiveReferences(k, s)
-    
-  predicate Apply2(k: Constants, s: Variables, s': Variables, op1: CacheOp, op2: CacheOp)
-    ensures Apply2(k, s, s', op1, op2) ==> ViewOf(k, s') == ApplyToView(ApplyToView(ViewOf(k, s), op1), op2)
-  {
-    exists sint ::
-      && Apply(k, s, sint, op1)
-      && Apply(k, sint, s', op2)
-  }
+  predicate Write<T>(k: Constants, s: Variables, s': Variables, ref: Reference, block: T, successors: iset<Reference>) {
+    && successors <= LiveReferences(k, s)
+    && ref in LiveReferences(k, s)
 
+    && s'.reftree == s.reftree[ref := successors]
+    && s'.view == s.view[ref := block]
+  }
+    
+  predicate Alloc<T>(k: Constants, s: Variables, s': Variables, block: T, successors: iset<Reference>, ref: Reference) {
+    && successors <= LiveReferences(k, s)
+    && ref !in LiveReferences(k, s)
+
+    && s'.reftree == s.reftree[ref := successors]
+    && s'.view == s.view[ref := block]
+  }
+    
   predicate GC(k: Constants, s: Variables, s': Variables, ref: Reference) {
     && ref !in LiveReferences(k, s)
-    && ref in ViewOf(k, s)
+    && ref in s.view
     && s'.view == IMapRemove(s.view, ref)
     && s'.reftree == s.reftree
   }
   
-  predicate Init(k: Constants, s: Variables)
+  predicate Init<T>(k: Constants, s: Variables, block: T) {
+    && s.view == imap[Root(k) := block]
+    && s.reftree == imap[Root(k) := iset{}]
+  }
+
+  datatype Step<T> =
+    | AllocStep(block: T, successors: iset<Reference>, ref: Reference)
+    | WriteStep(ref: Reference, block: T, successors: iset<Reference>)
+    | GCStep(ref: Reference)
+
+  predicate NextStep(k: Constants, s: Variables, s': Variables, step: Step) {
+    match step {
+      case AllocStep(block, successors, ref) => Alloc(k, s, s', block, successors, ref)
+      case WriteStep(ref, block, successors) => Write(k, s, s', ref, block, successors)
+      case GCStep(ref) => GC(k, s, s', ref)
+    }
+  }
+    
+  predicate Next<T(!new)>(k: Constants, s: Variables, s': Variables) {
+    exists step :: NextStep(k, s, s', step)
+  }
+    
+  /////////// Invariants
+
+  predicate Inv(k: Constants, s: Variables) {
+    && LiveDataAvailable(k, s)
+  }
+
+  lemma AllocPreservesInvariant<T>(k: Constants, s: Variables, s': Variables, block: T, successors: iset<Reference>, ref: Reference)
+    requires Inv(k, s)
+    requires Alloc(k, s, s', block, successors, ref)
+    ensures Inv(k, s')
+  {
+  }
+  
 }
